progress on shortest path verification and changing the type of the C parent edge

shortest_path_checker.c
@@ -16,8 +16,15 @@ typedef struct IGraph {
 
 typedef struct EInt {
 	unsigned int val;
-	unsigned int isInf;
+	unsigned int isInf; 
+// isInf is meant to be a boolean value. For enu and dist it flags if they are unreachable
 } EInt;
+
+typedef struct OInt {
+	unsigned int val;
+	unsigned int none; 
+// For pred none used to denote that the parent edge does not exist (i.e. unreachable or source vertex)
+} OInt;
 // Abbreviations
 
 #define ivertex_cnt(g) g->num_vertices
@@ -45,19 +52,22 @@ int trian(IGraph *g, EInt *dist, unsigned int *c) {
 	return 1;
 }
 
-int just(IGraph *g, EInt *dist, unsigned int *c, unsigned int s, EInt *enu, int *pred) {
+int just(IGraph *g, EInt *dist, unsigned int *c, unsigned int s, EInt *enu, OInt *pred) {
 	unsigned int edge_id;
 	for(unsigned int v = 0; v < ivertex_cnt(g); v++) {
-		edge_id = pred[v];
+		edge_id = pred[v].val;
 		if(v != s) {
+		 if (pred[v].none !=0)
+		 {
 			//if(enu[v] >= 0) {
-     if(enu[v].isInf != 0) {
+      if(enu[v].isInf != 0) {
 				if(edge_id >= iedge_cnt(g)) return 0;
 				if(iarcs(g, edge_id).second != v) return 0;
 				if(dist[v].val != dist[iarcs(g, edge_id).first].val + c[edge_id]) return 0;
 				if(enu[v].val != enu[iarcs(g, edge_id).first].val + 1) return 0; // onum
 			}
 		}
+	 }
 	}
 	return 1;
 }
@@ -81,7 +91,7 @@ int no_path(IGraph *g, EInt *dist, EInt *enu) {
 	// return 1;
 // }
 
-int check_basic_just_sp(IGraph *g, EInt *dist, unsigned int *c, unsigned int s, EInt *enu, int *pred) {
+int check_basic_just_sp(IGraph *g, EInt *dist, unsigned int *c, unsigned int s, EInt *enu, OInt *pred) {
 	if(!is_wellformed(g)) return 0;
 	if(dist[s].val != 0)
    { if (dist[s].isInf == 0) return 0; }
@@ -90,7 +100,7 @@ int check_basic_just_sp(IGraph *g, EInt *dist, unsigned int *c, unsigned int s, 
 	return 1;
 }
 
-int check_sp(IGraph *g, EInt *dist, unsigned int *c, unsigned int s, EInt *enu, int *pred) {
+int check_sp(IGraph *g, EInt *dist, unsigned int *c, unsigned int s, EInt *enu, OInt *pred) {
 	if(!check_basic_just_sp(g, dist, c, s, enu, pred)) return 0;
 	if(s >= ivertex_cnt(g)) return 0;
 	if(dist[s].val != 0) return 0;
